coq/TypedSyntaxProperties.v
@@ -1,0 +1,52 @@
+Require Import Koika.TypedSyntaxTools Koika.Semantics.
+
+Section TypedSyntaxProperties.
+  Context {pos_t var_t rule_name_t reg_t ext_fn_t: Type}.
+  Context {reg_t_eq_dec: EqDec reg_t}.
+
+  Context {R: reg_t -> type}.
+  Context {Sigma: ext_fn_t -> ExternalSignature}.
+
+  Context {REnv: Env reg_t}.
+  Context (r: REnv.(env_t) R).
+  Context (sigma: forall f, Sig_denote (Sigma f)).
+
+  Notation rule := (rule pos_t var_t R Sigma).
+  Notation action := (action pos_t var_t R Sigma).
+  Notation scheduler := (scheduler pos_t rule_name_t).
+  Notation Log := (Log R REnv).
+
+  Lemma bits_to_N_zero:
+    forall (tau : type) (cst : tau),
+      N.eqb (Bits.to_N (bits_of_value cst)) N.zero = true ->
+      bits_of_value cst = Bits.zeroes (type_sz tau).
+  Proof.
+    intros * Heq%Neqb_ok.
+    apply Bits.to_N_inj.
+    rewrite Bits.to_N_zeroes.
+    assumption.
+  Qed.
+
+  Lemma is_const_zero_correct {sig tau} :
+    forall (a: action sig tau) (Gamma: vcontext sig) (sched_log: Log) (action_log: Log),
+      is_const_zero a = true ->
+      match interp_action r sigma Gamma sched_log action_log a with
+      | Some (_, v, _) => bits_of_value v = Bits.zeroes (type_sz tau)
+      | None => True
+      end.
+  Proof.
+    induction a; cbn; intros; try discriminate;
+      repeat match goal with
+             | [ H: (forall Gamma L l, _ -> match interp_action ?r ?sigma Gamma L l ?a with _ => _ end)
+                 |- context[interp_action ?r ?sigma ?Gamma ?L ?l ?a] ] =>
+               specialize (H Gamma L l)
+             | [ H: is_const_zero ?x = true -> _, H': is_const_zero ?x = true |- _ ] =>
+               specialize (H H')
+             | [  |- context[opt_bind (interp_action ?r ?sigma ?Gamma ?sched_log ?action_log ?a) _] ] =>
+               destruct (interp_action r sigma Gamma sched_log action_log a) as [ ((? & ?) & ?) | ]
+             | [ H: _ && _ = _ |- _ ] => apply andb_prop in H; destruct H
+             | [  |- context[if ?c then _ else _] ] => destruct c
+             | _ => eauto using bits_to_N_zero || simpl
+             end.
+  Qed.
+End TypedSyntaxProperties.
